src/program_proof/simplepb/pb_preread_protocol.v
@@ -1,35 +1,47 @@
 From Perennial.program_proof Require Import grove_prelude.
 From Goose.github_com.mit_pdos.gokv.simplepb Require Export pb.
 From iris.base_logic Require Export lib.ghost_var mono_nat.
-From iris.algebra Require Import auth dfrac_agree mono_list csum gset.
+From iris.algebra Require Import auth dfrac_agree mono_list csum gset gmap_view.
 From Perennial.program_proof.simplepb Require Import pb_protocol.
 From Perennial.Helpers Require Import ListSolver.
+From Perennial.base_logic Require Import lib.saved_prop.
 
 Section pb_preread_protocol.
-(* Use (authR gsetR) for monotonic sets. *)
 
 Context `{EntryType:Type}.
-Context `{pb_ghostG EntryType Σ}.
-Context `{invGS Σ}.
 
-(* FIXME: this is not actually countable. This is a requirement from gset, but
-   feels like it shouldn't really be needed. We can make do by having a list
-   instead of gset, and ignore the ordering.
- *)
-Context `{Countable (list EntryType → iProp Σ)}.
+Class pb_prereadG Σ :=
+  {
+    preread_pb_ghostG :> pb_ghostG (EntryType:=EntryType) Σ ;
+    preread_gnameMapG :> inG Σ (authR (gmapUR nat (mono_listR (leibnizO gname)))) ;
+    preread_savedG :> savedPredG Σ (list EntryType)
+  }.
+
+Context `{invGS Σ}.
+Context `{pb_prereadG Σ}.
 
 (* This is the key ghost state, keeping track of RO ops that have been
    pre-applied before state is committed. *)
-Implicit Types ros:gmap nat (gset (list EntryType → iProp Σ)).
+(* XXX: the "list" of (list EntryType → iProp Σ) is really meant to be a gset,
+   but can't have a gset of iProp Σ. *)
+Implicit Types ros:gmap nat (list (list EntryType → iProp Σ)).
 
-Definition own_proposed_reads (γ:gname) (ros:gmap nat (gset (list EntryType → iProp Σ))) : iProp Σ.
-Admitted.
+Definition own_proposed_reads (γ:gname) (ros:gmap nat (list (list EntryType → iProp Σ))) : iProp Σ :=
+  ∃ (rosγ:gmap nat (list gname)),
+  own γ (●((λ rosγAtIdx, ●ML rosγAtIdx) <$> rosγ) : auth (gmap nat (mono_listR (leibnizO gname)))) ∗
+  ([∗ map] idx ↦ rosAtIdx ; rosγAtIdx ∈ ros ; rosγ,
+    [∗ list] _ ↦ γprop ; Q ∈ rosγAtIdx ; rosAtIdx, saved_pred_own γprop DfracDiscarded Q)
+.
 
-Definition is_proposed_read (γ:gname) (idx:nat) (Q:(list EntryType → iProp Σ)) : iProp Σ.
-Admitted.
+Definition is_proposed_read (γ:gname) (idx:nat) (Q:(list EntryType → iProp Σ)) : iProp Σ :=
+  ∃ rosγAtIdx γprop,
+  own γ (◯{[ idx := ◯ML rosγAtIdx ]}) ∗
+  ⌜γprop ∈ rosγAtIdx⌝ ∗
+  saved_pred_own γprop DfracDiscarded Q
+.
 
 Instance is_proposed_read_pers γ idx Q : Persistent (is_proposed_read γ idx Q).
-Admitted.
+Proof. apply _. Qed.
 
 (* This is a 1/2 fraction *)
 Definition own_log (γlog:gname) (σ:list EntryType) : iProp Σ :=
@@ -40,18 +52,19 @@ Definition is_log_lb (γlog:gname) (σ:list EntryType) : iProp Σ :=
 
 (* Maybe make the fupds non-persistent, and track things more carefully in the
    proof. *)
+
+Definition prereadN := nroot .@ "preread".
+
 Definition have_proposed_reads_fupds γlog ros : iProp Σ :=
-  [∗ map] idx ↦ rosAtIdx ∈ ros, [∗ set] Q ∈ rosAtIdx,
-    □(|={⊤,∅}=> ∃ σ, own_log γlog σ ∗ (own_log γlog σ ={∅,⊤}=∗ □ Q σ))
+  [∗ map] idx ↦ rosAtIdx ∈ ros, [∗ list] Q ∈ rosAtIdx,
+    □(|={⊤∖↑prereadN,∅}=> ∃ σ, own_log γlog σ ∗ (own_log γlog σ ={∅,⊤∖↑prereadN}=∗ □ Q σ))
 .
 
 (* Maybe make Q not persistent, and escrow it back to the caller *)
 Definition have_completed_reads_Qs ros σ : iProp Σ :=
-  [∗ map] idx ↦ rosAtIdx ∈ ros, ⌜idx <= length σ⌝ → [∗ set] Q ∈ rosAtIdx,
+  [∗ map] idx ↦ rosAtIdx ∈ ros, ⌜idx <= length σ⌝ → [∗ list] Q ∈ rosAtIdx,
     □ Q (take idx σ)
 .
-
-Definition prereadN := nroot .@ "preread".
 
 Definition preread_inv γ γlog γreads : iProp Σ :=
   inv prereadN (
@@ -65,12 +78,34 @@ Definition preread_inv γ γlog γreads : iProp Σ :=
   )
 .
 
-Lemma update_map_fmset idx Q ros γreads :
+Lemma update_map_mset_ipred idx Q ros γreads :
   own_proposed_reads γreads ros ==∗
-  own_proposed_reads γreads (<[ idx := {[ Q ]} ∪ default ∅ (ros !! idx) ]> ros)
+  own_proposed_reads γreads (<[ idx := (default [] (ros !! idx)) ++ [Q] ]> ros)
 .
 Proof.
-Admitted.
+  iIntros "Hown".
+  iDestruct "Hown" as (?) "[Hown Hrest]".
+  iMod (saved_pred_alloc Q DfracDiscarded) as (γpred) "#Hpred".
+  { done. }
+  iExists _.
+  iMod (own_update with "Hown") as "$".
+  {
+    instantiate (1:=<[idx:=default [] (ros !! idx) ++ [γpred]]> rosγ ).
+    rewrite fmap_insert.
+    About auth_update.
+
+    (* FIXME *)
+    Need to fix the resource algebra monotonic map of sets of iPredicates.
+    Maybe take inspiration from how mono_listR works, by using auth but
+    making the mono_list_auth contain an auth and a frag.
+    (* ***** *)
+
+    apply auth_update.
+    Search gmap_view_auth.
+    Search gmapR.
+    apply insert_update.
+  }
+Qed.
 
 Lemma map_fmset_get_elem idx Q ros γreads :
   Q ∈ default ∅ (ros !! idx) →
@@ -113,14 +148,13 @@ Proof.
 Qed.
 
 Lemma start_read_step Q γ γlog γreads idx σ :
-  idx > length σ →
+  idx >= length σ →
   £ 1 -∗
   preread_inv γ γlog γreads -∗
-  □(|={⊤,∅}=> ∃ σ, own_log γlog σ ∗ (own_log γlog σ ={∅,⊤}=∗ □ Q σ)) -∗
-  own_log γlog σ (* FIXME: maybe own_commit instead of own_log? Whatever this
-                    resource is will come from the own_lease. *)
-  ={↑prereadN}=∗
-  is_proposed_read γreads idx Q ∗ own_log γlog σ
+  □(|={⊤∖↑prereadN,∅}=> ∃ σ, own_log γlog σ ∗ (own_log γlog σ ={∅,⊤∖↑prereadN}=∗ □ Q σ)) -∗
+  own_commit γ σ
+  ={⊤}=∗
+  is_proposed_read γreads idx Q ∗ own_commit γ σ
 .
 Proof.
   intros Hidx.
@@ -128,9 +162,18 @@ Proof.
   iInv "Hinv" as "Hown" "Hclose".
   iMod (lc_fupd_elim_later with "Hlc Hown") as "Hown".
   iNamed "Hown".
-  iDestruct (own_log_agree with "Hlog_in Hlog") as %?.
+  iDestruct (own_log_agree with "Hlog_in HpbLog") as %?.
   subst.
   iFrame "Hlog_in".
+
+  (* we'll fire the fupd here for the case that idx = length σ, and later might
+     decide to throw away the Q *)
+  iAssert (_) with "Hupd" as "Hupd2".
+  iMod "Hupd2" as (?) "[Hlog2 Hupd2]".
+  iDestruct (own_log_agree with "Hlog2 Hlog") as %?.
+  subst.
+  iMod ("Hupd2" with "Hlog2") as "#?".
+
   iMod (update_map_fmset idx Q with "HownRos") as "HownRos".
   iDestruct (map_fmset_get_elem idx Q with "HownRos") as "#His_read".
   { rewrite lookup_insert. set_solver. }
@@ -155,6 +198,24 @@ Proof.
   simpl.
   iApply (big_sepM_insert_2 with "[] HcompletedRead").
   iIntros (?).
+  destruct (decide (idx = length σ0)).
+  {
+    subst.
+    iApply big_sepS_union_2.
+    {
+      iApply big_sepS_singleton.
+      iModIntro.
+      by rewrite firstn_all.
+    }
+    (* again, the rest of these follow from the previous Q's. *)
+    destruct (ros !! (length σ0)) as [] eqn:Hlookup.
+    {
+      iDestruct (big_sepM_lookup with "HcompletedRead") as "Hupds".
+      { done. }
+      by iApply "Hupds".
+    }
+    by iApply big_sepS_empty.
+  }
   exfalso.
   lia.
 Qed.
@@ -189,7 +250,19 @@ Proof.
   iExactEq "H2".
   repeat f_equal.
   (* TODO: list_solver *)
-  admit.
-Admitted.
+  subst.
+  destruct Hprefix as []; subst.
+  apply take_app.
+Qed.
+
+(*
+Lemma propose_rw_op_valid op γ γlog γreads :
+  £ 1 -∗
+  preread_inv γ γlog γreads -∗
+  □(|={⊤∖↑prereadN,∅}=> ∃ σ, own_log γlog σ ∗ (own_log γlog (σ ++ [op]) ={∅,⊤∖↑prereadN}=∗ True))
+  ={↑prereadN}=∗
+  (|={⊤∖↑ghostN,∅}=> ∃ someσ, own_ghost γ someσ ∗ (⌜someσ = σ⌝ -∗ own_ghost γ (someσ ++ [op]) ={∅,⊤∖↑ghostN}=∗ True))
+.
+Proof. *)
 
 End pb_preread_protocol.
